theories/Semantics/Type_System.v
@@ -1,213 +1,103 @@
-From Coq Require Import Lia Arith.PeanoNat Classes.Morphisms List.
-From DeBrLevel Require Import ListLevel LevelInterface.
-From Mecha Require Import Typ Resource Term Var VContext Resources.
-Import ResourceNotations TypNotations TermNotations ListNotations
+From Coq Require Import Lia Arith.PeanoNat Classes.Morphisms.
+From Mecha Require Import Typ Resource Term Var VContext RContext Resources.
+Import ResourceNotations TypNotations TermNotations RContextNotations 
        VContextNotations VarNotations ResourcesNotations SetNotations.
 
 
 (** * Semantics - Type System 
 
-  Wormhole's type system, denoted Γ ⋅ RC.t ⊢ t ∈ α, ensures that [t] is typed by [α] under two contexts [Γ] and [RC.t]. The former is the usual variable context, defined in [VContext.v], and the latter is a resource context, defined in [RContext.v]. This file contains the [well_typed] property definition and its weakening proofs.
+  Wormhole's type system, denoted Γ ⋅ ℜ ⊢ t ∈ α, ensures that [t] is typed by [α] under two contexts [Γ] and [ℜ]. The former is the usual variable context, defined in [VContext.v], and the latter is a resource context, defined in [RContext.v]. This file contains the [well_typed] property definition and its weakening proofs.
 *)
 
 
+Open Scope rcontext_scope. 
 
-Module RC <: IsLvlETWL.
-  Include IsLvlListETWL PairTyp.
-
-  Definition threshold (l :t) := List.length l.
-
-  Definition find (n : nat) (l : t) := List.nth_error l n.
-
-  Definition add v (l : t) := l ++ [v].
-
-  Definition multi_add vl (l : t) :=
-    List.fold_right (fun v acc => add v acc) l vl.
-
-  Definition key_in n (l : t) := n < (threshold l).
-
-  Lemma find_some_in n v l :
-    find n l = Some v -> key_in n l.
-  Proof.
-    revert n.
-    induction l; intros n Hfi.
-    - unfold key_in, find in *; simpl in *.
-      destruct n; simpl in *; inversion Hfi.
-    - destruct n; simpl in *.
-      -- unfold key_in; simpl; lia.
-      -- unfold key_in; simpl.
-         apply IHl in Hfi; unfold key_in in *; lia.
-  Qed.
-
-  Lemma find_some_In n v l :
-    find n l = Some v -> In v l.
-  Proof.
-    revert n.
-    induction l; intros n Hfi.
-    - unfold key_in, find in *; simpl in *.
-      destruct n; simpl in *; inversion Hfi.
-    - destruct n; simpl in *.
-      -- inversion Hfi; auto.
-      -- apply IHl in Hfi; auto.
-  Qed.
-
-  Lemma key_in_add n v l :
-    key_in n (add v l) -> n = threshold l \/ key_in n l.
-  Proof.
-    unfold key_in, threshold, add.
-    rewrite List.length_app; simpl in *.
-    lia.
-  Qed.
-
-  Lemma threshold_add v l : threshold (add v l) = S (threshold l).
-  Proof.
-    unfold threshold, add.
-    rewrite List.length_app; simpl in *.
-    lia.
-  Qed.
-
-  Lemma Wf_add n v l :
-    Wf n (add v l) -> PairTyp.Wf n v /\ Wf n l.
-  Proof.
-    intro Hwf; split.
-    - apply Hwf; unfold add.
-      apply in_or_app; right; simpl; auto.
-    - intros x HIn; apply Hwf.
-      unfold add.
-      apply in_or_app; left; simpl; auto.
-  Qed.
-
-  Lemma Wf_add' n v l :
-    PairTyp.Wf n v /\ Wf n l -> Wf n (add v l).
-  Proof.
-    intros [Hwfv Hwf] x HIn.
-    unfold add in *.
-    apply in_app_or in HIn as [].
-    - now apply Hwf.
-    - simpl in *; destruct H; try contradiction; subst; auto.
-  Qed.
-
-  Lemma Wf_add_iff n v l :
-    Wf n (add v l) <-> PairTyp.Wf n v /\ Wf n l.
-  Proof.
-    split.
-    - apply Wf_add.
-    - apply Wf_add'.
-  Qed.
-
-  Lemma find_Wf n v l : 
-    Wf (threshold l) l ->
-    find n l = Some v -> Resource.Wf (threshold l) n /\ PairTyp.Wf (threshold l) v.
-  Proof.
-    unfold Wf.
-    intros Hwf Hfi.
-    apply find_some_in in Hfi as Hin.
-    apply find_some_In in Hfi as HIn.
-    apply Hwf in HIn; split; auto.
-  Qed.
-
-  Lemma Wf_wh v v' (l : t) :
-    Wf (threshold l) l -> (threshold l ⊩ v)%pty -> (threshold l ⊩ v')%pty -> 
-    Wf (S (S (threshold l))) (add v (add v' l)).
-  Proof.
-    intros Hvm Hvv Hvv'.
-    repeat rewrite Wf_add_iff.
-    split.
-    - apply PairTyp.Wf_weakening with (n := threshold l); auto.
-    - split.
-      -- apply PairTyp.Wf_weakening with (n := threshold l); auto.
-      -- apply Wf_weakening with (k := threshold l); auto.
-  Qed.
-          
-End RC.
-
+Module RC := RContext.
 Module VC := VContext.
 
 (** ** Definition - Type System *)
 
 Reserved Notation "G '⋅' R '⊢' t '∈' T" (at level 40, t custom wh, T custom wh).
 
-Inductive well_typed : Γ -> RC.t -> Λ -> Τ -> Prop :=
-  | wt_var (Γ : Γ) (Re : RC.t) (x : variable) (τ : Τ) :
+Inductive well_typed : Γ -> ℜ -> Λ -> Τ -> Prop :=
+  | wt_var (Γ : Γ) (Re : ℜ) (x : variable) (τ : Τ) :
 
             (Γ ⌊x⌋)%vc = Some τ -> 
     (* -------------------------------- WT-Var *)
          Γ ⋅ Re ⊢ {Term.tm_var x} ∈ τ
 
-  | wt_abs (Γ : Γ) (Re : RC.t) (x : variable) (t : Λ) (α β : Τ) :
+  | wt_abs (Γ : Γ) (Re : ℜ) (x : variable) (t : Λ) (α β : Τ) :
 
-         (⌈x ⤆ α⌉ Γ)%vc ⋅ Re ⊢ t ∈ β -> 
-         ((RC.threshold Re) ⊩ α)%ty ->
+         (⌈x ⤆ α⌉ Γ)%vc ⋅ Re ⊢ t ∈ β -> (Re⁺ ⊩ α)%ty ->
     (* --------------------------------------------------- WT-Abs *)
                   Γ ⋅ Re ⊢ (\x, t) ∈ (α → β)
 
-  | wt_app  (Γ : Γ) (Re : RC.t) (t1 t2 : Λ) (α β : Τ) :
+  | wt_app  (Γ : Γ) (Re : ℜ) (t1 t2 : Λ) (α β : Τ) :
 
          Γ ⋅ Re ⊢ t1 ∈ (α → β) -> Γ ⋅ Re ⊢ t2 ∈ α -> 
     (* ------------------------------------------------ WT-App *)
                       Γ ⋅ Re ⊢ t1 t2 ∈ β
 
-  | wt_unit (Γ : Γ) (Re : RC.t) :
+  | wt_unit (Γ : Γ) (Re : ℜ) :
 
     (* --------------------- WT-Unit *)
          Γ ⋅ Re ⊢ unit ∈ 𝟙       
 
-  | wt_pair (Γ : Γ) (Re : RC.t) (t1 t2 : Λ) (α β : Τ) :
+  | wt_pair (Γ : Γ) (Re : ℜ) (t1 t2 : Λ) (α β : Τ) :
 
          Γ ⋅ Re ⊢ t1 ∈ α -> Γ ⋅ Re ⊢ t2 ∈ β -> 
     (* ------------------------------------------ WT-Pair *)
             Γ ⋅ Re ⊢ ⟨t1, t2⟩ ∈ (α × β)
 
-  | wt_fst (Γ : Γ) (Re : RC.t) (t : Λ) (α β : Τ) :
+  | wt_fst (Γ : Γ) (Re : ℜ) (t : Λ) (α β : Τ) :
 
          Γ ⋅ Re ⊢ t ∈ (α × β) -> 
     (* --------------------------- WT-Fst *)
           Γ ⋅ Re ⊢ (fst.t) ∈ α
 
-  | wt_snd (Γ : Γ) (Re : RC.t) (t : Λ) (α β : Τ) :
+  | wt_snd (Γ : Γ) (Re : ℜ) (t : Λ) (α β : Τ) :
 
         Γ ⋅ Re ⊢ t ∈ (α × β) -> 
     (* --------------------------- WT-Snd *)
           Γ ⋅ Re ⊢ (snd.t) ∈ β
 
-  | wt_fix (Γ : Γ) (Re : RC.t) (t : Λ) (τ : Τ) :
+  | wt_fix (Γ : Γ) (Re : ℜ) (t : Λ) (τ : Τ) :
 
          Γ ⋅ Re ⊢ t ∈ (τ → τ) ->
     (* --------------------------- WT-Fix *)
            Γ ⋅ Re ⊢ Fix t ∈ τ
 
-  | wt_arr (Γ : Γ) (Re : RC.t) (t : Λ) (α β : Τ) :
+  | wt_arr (Γ : Γ) (Re : ℜ) (t : Λ) (α β : Τ) :
 
              Γ ⋅ Re ⊢ t ∈ (α → β) -> 
     (* ------------------------------------- WT-Arr *)
          Γ ⋅ Re ⊢ arr(t) ∈ (α ⟿ β ∣ ∅)%s
 
-  | wt_first (Γ : Γ) (Re : RC.t) (R : resources) (t : Λ) (α β τ : Τ) :
+  | wt_first (Γ : Γ) (Re : ℜ) (R : resources) (t : Λ) (α β τ : Τ) :
 
-         Γ ⋅ Re ⊢ t ∈ (α ⟿ β ∣ R) -> 
-         ((RC.threshold Re) ⊩ τ)%ty ->
+         Γ ⋅ Re ⊢ t ∈ (α ⟿ β ∣ R) -> (Re⁺ ⊩ τ)%ty ->
     (* ------------------------------------------------ WT-First *)
          Γ ⋅ Re ⊢ first(t) ∈ ((α × τ) ⟿ (β × τ) ∣ R)
 
-  | wt_comp (Γ : Γ) (Re : RC.t) (R R1 R2 : resources) (t1 t2 : Λ) (α β τ : Τ) :
+  | wt_comp (Γ : Γ) (Re : ℜ) (R R1 R2 : resources) (t1 t2 : Λ) (α β τ : Τ) :
 
          Γ ⋅ Re ⊢ t1 ∈ (α ⟿ τ ∣ R1) -> (R = (R1 ∪ R2))%s -> 
          Γ ⋅ Re ⊢ t2 ∈ (τ ⟿ β ∣ R2) -> (∅ = (R1 ∩ R2))%s -> 
     (* -------------------------------------------------------- WT-Comp *)
               Γ ⋅ Re ⊢ (t1 >>> t2) ∈ (α ⟿ β ∣ R)
 
-  | wt_rsf (Γ : Γ) (Re : RC.t) (r : resource) (τin τout : Τ) :
+  | wt_rsf (Γ : Γ) (Re : ℜ) (r : resource) (τin τout : Τ) :
 
-              RC.find r Re = Some (τin,τout) ->
+              Re ⌊r⌋ = Some (τin,τout) ->
     (* -------------------------------------------- WT-Rsf *)
          Γ ⋅ Re ⊢ rsf[r] ∈ (τin ⟿ τout ∣ \{{r}})
 
-  | wt_wh (Γ : Γ) (Re : RC.t) (R R' : resources) (t1 t2 : Λ) (α β τ : Τ) :
+  | wt_wh (Γ : Γ) (Re : ℜ) (R R' : resources) (t1 t2 : Λ) (α β τ : Τ) :
 
-         (R = R' \ \{{ (RC.threshold Re); (S ((RC.threshold Re))) }})%s -> ((RC.threshold Re) ⊩ α)%ty -> ((RC.threshold Re) ⊩ β)%ty ->
+         (R = R' \ \{{ Re⁺; (S (Re⁺)) }})%s -> (Re⁺ ⊩ α)%ty -> (Re⁺ ⊩ β)%ty ->
 
          Γ ⋅ Re ⊢ t1 ∈ τ ->
-         Γ ⋅ (RC.add (τ,<[𝟙]>) (RC.add (<[𝟙]>,τ) Re)) ⊢ t2 ∈ (α ⟿ β ∣ R') ->
+         Γ ⋅ (⌈(S (Re⁺)) ⤆ (τ,<[𝟙]>)⌉ (⌈Re⁺ ⤆ (<[𝟙]>,τ)⌉ Re)) ⊢ t2 ∈ (α ⟿ β ∣ R') ->
     (* -------------------------------------------------------------------------------- WT-Wh *)
                           Γ ⋅ Re ⊢ wormhole(t1;t2) ∈ (α ⟿ β ∣ R)
 
@@ -225,26 +115,39 @@ Open Scope term_scope.
   Proper (VC.eq ==> RC.eq ==> Term.eq ==> Typ.eq ==> iff) well_typed.
 Proof.
   intros Γ Γ' HGeq Re Re1 HReq t' t HTmeq α β HTyeq.
-  unfold Term.eq,Typ.eq,RC.eq in *; subst; split.
-  - intro wt; revert Γ' HGeq; induction wt; intros; eauto.
+  unfold Term.eq,Typ.eq in *; subst; split.
+  - intro wt; revert Γ' HGeq Re1 HReq; induction wt; intros; eauto.
     -- constructor; now rewrite <- HGeq.
-    -- constructor; auto.
+    -- rewrite HReq in *; constructor; auto.
        apply IHwt; auto; now rewrite HGeq.
-  - intro wt; revert Γ HGeq; induction wt; intros; eauto.
+    -- constructor; auto; now rewrite <- HReq.
+    -- constructor; auto; now rewrite <- HReq.
+    -- apply wt_wh with (R' := R') (τ := τ); auto;
+       try (apply IHwt2; auto); now rewrite <- HReq.
+  - intro wt; revert Γ HGeq Re HReq; induction wt; intros; eauto.
     -- constructor; now rewrite HGeq.
-    -- constructor; auto.
+    -- rewrite <- HReq in *; constructor; auto.
        apply IHwt; auto; now rewrite <- HGeq.
+    -- constructor; auto; now rewrite HReq.
+    -- constructor; auto; now rewrite HReq.
+    -- apply wt_wh with (R' := R') (τ := τ); auto;
+       try (apply IHwt2; auto); now rewrite HReq.
 Qed.
+
+Lemma wt_deterministic (Γ : Γ) (Re : ℜ) (t : Λ) (α β : Τ) :
+  Γ ⋅ Re ⊢ t ∈ α -> Γ ⋅ Re ⊢ t ∈ β -> α = β.
+Proof.
+Abort.
 
 (** *** Used resource names come from the resource context
 
   Suppose a value [t] (1), well typed by [(α ⟿ β ∣ R)] under contexts [Γ] and [Re] (2). Resource names in the set of used resources [R] have to be in Re, i.e. We can use only resource names known.
 *)
-Theorem typing_Re_R (Γ : Γ) (Re : RC.t) (t : Λ) (α β : Τ) (R : resources) :
+Theorem typing_Re_R (Γ : Γ) (Re : ℜ) (t : Λ) (α β : Τ) (R : resources) :
 
        (* (1) *) value(t) -> (* (2) *) Γ ⋅ Re ⊢ t ∈ (α ⟿ β ∣ R) -> 
   (* ---------------------------------------------------------------- *)
-           (forall (r : resource), (r ∈ R)%s -> (RC.key_in r Re)).
+           (forall (r : resource), (r ∈ R)%s -> (r ∈ Re)%rc).
 Proof.
   revert Γ Re α β R; induction t; intros Γ Re α β R Hvt Hwt r1 HIn; 
   inversion Hvt; subst; inversion Hwt; subst.
@@ -254,7 +157,7 @@ Proof.
   - apply (IHt Γ _ α0 β0 R); assumption.
   (* rsf *)
   - rewrite Resources.St.singleton_spec in HIn; subst.
-    apply RC.find_some_in in H3; auto.
+    exists (α,β); now apply RC.find_2.
   (* comp *)
   - rewrite H9 in HIn. 
     apply Resources.St.union_spec in HIn as [HIn | HIn]; eauto.
@@ -263,21 +166,19 @@ Proof.
     apply Resources.St.diff_spec in HIn as [HIn HnIn].
     eapply IHt2 in H12; eauto. 
     (repeat rewrite Resources.St.add_notin_spec in HnIn); destruct HnIn as [Hneq [Hneq' _]].
-    apply RC.key_in_add in H12 as [].
-    -- rewrite RC.threshold_add in H; subst; contradiction.
-    -- apply RC.key_in_add in H as []; auto.
-       subst; contradiction.
+    (repeat rewrite RC.add_in_iff in H12). 
+    destruct H12 as [Heq | [Heq | HIn']]; subst; try contradiction; assumption. 
 Qed.
 
 (** *** Well typed implies well formedness 
 
-  Suppose a term [t], well typed by [τ] under contexts [Γ] and [Re] (3), knowing that both contexts are well formed under [(RC.threshold Re)] (1,2). We can prove that [t] and [τ] are also well formed under [(RC.threshold Re)] (4,5).
+  Suppose a term [t], well typed by [τ] under contexts [Γ] and [Re] (3), knowing that both contexts are well formed under [Re⁺] (1,2). We can prove that [t] and [τ] are also well formed under [Re⁺] (4,5).
 *)
-Theorem well_typed_implies_Wf (Γ : Γ) (Re : RC.t) (t : Λ) (τ : Τ) :
+Theorem well_typed_implies_Wf (Γ : Γ) (Re : ℜ) (t : Λ) (τ : Τ) :
 
-       (* (1) *) ((RC.threshold Re) ⊩ Γ)%vc ->  (* (2) *) (RC.Wf (RC.threshold Re) Re) -> (* (3) *) Γ ⋅ Re ⊢ t ∈ τ ->
+       (* (1) *) (Re⁺ ⊩ Γ)%vc ->  (* (2) *) (Re⁺ ⊩ Re)%rc -> (* (3) *) Γ ⋅ Re ⊢ t ∈ τ ->
   (* -------------------------------------------------------------------------------------- *)
-                      (* (4) *) (RC.threshold Re) ⊩ t /\ (* (5) *) ((RC.threshold Re) ⊩ τ)%ty.
+                      (* (4) *) Re⁺ ⊩ t /\ (* (5) *) (Re⁺ ⊩ τ)%ty.
 Proof.
   revert Γ Re τ; induction t; simpl; intros Γ Re τ HvΓ HvRe Hwt; inversion Hwt; subst;
   try (apply IHt in H2 as [Hvt Hvf]; auto; inversion Hvf; subst; now repeat constructor).
@@ -285,7 +186,7 @@ Proof.
   - repeat constructor.
   (* variable *)
   - split; try constructor. 
-    now apply (VC.Wf_find ((RC.threshold Re))) in H2.
+    now apply (VC.Wf_find (Re⁺)) in H2.
   (* abstraction *)
   - apply (IHt (⌈x ⤆ α⌉ Γ)%vc _ β) in HvRe as [Hvt Hvf]; auto.
     -- split; auto; constructor; assumption.
@@ -302,7 +203,7 @@ Proof.
   - apply IHt in H0 as [Hvt Hvf]; auto; inversion Hvf; subst.
     repeat constructor; auto.
   (* rsf *)
-  - apply RC.find_Wf in H2 as [Hvr Hvf]; auto.
+  - apply RC.Wf_find with (lb := Re⁺) in H2 as [Hvr Hvf]; auto.
     inversion Hvf; simpl in *; repeat constructor; auto.
     now apply Resources.Wf_singleton_iff.
   (* comp *)
@@ -311,12 +212,10 @@ Proof.
     rewrite H2; rewrite Resources.Wf_union_iff; now split.
   (* wormhole *)
   - apply IHt1 in H6 as [Hvt1 Hvτ]; auto.
-    apply IHt2 in H8 as [Hvt2 Hvf]; repeat (rewrite RC.threshold_add in *).
-    -- inversion Hvf; subst. 
-       split; constructor; auto.
-       apply Resources.eq_leibniz in H1; subst.
-       now apply Resources.Wf_wh.
-    -- apply VC.Wf_weakening with (k := (RC.threshold Re)); auto.
+    apply IHt2 in H8 as [Hvt2 Hvf]; rewrite RC.new_key_wh in *.
+    -- inversion Hvf; subst; repeat constructor; auto. 
+       rewrite H1; now apply Resources.Wf_wh.
+    -- apply VC.Wf_weakening with (k := Re⁺); auto.
     -- apply RC.Wf_wh; auto; now repeat constructor; simpl.
 Qed.
 
@@ -324,7 +223,7 @@ Qed.
 
   Suppose a term [t], well typed by [τ] under contexts [Γ] and [Re] (2) and another variable context named [Γ'] such as [Γ] is included in [Γ'] (1). We can state that [t] is also well typed by swap [Γ] with [Γ'].
 *)
-Theorem weakening_Γ (Γ Γ' : Γ) (Re : RC.t) (t : Λ) (τ : Τ) :
+Theorem weakening_Γ (Γ Γ' : Γ) (Re : ℜ) (t : Λ) (τ : Τ) :
 
        (* (1) *) (Γ ⊆ Γ')%vc -> (* (2) *) Γ ⋅ Re ⊢ t ∈ τ -> 
   (* -------------------------------------------------------- *)
@@ -344,16 +243,12 @@ Open Scope typ_scope.
   Suppose a term [t], well typed by [τ] under contexts [Γ] and [Re] (5) and another resource context named [Re1] such as ([[⧐ k – (k' - k)] Re]) is included in [Re1] (4). [k] and [k'] are levels such as they satisfy hypothesis (1),(2) and (3). We prove that [t] is also well typed by swap [Re] with [Re1] modulo [shift] applications.
   
 *)
-Theorem weakening_RC_gen (k k' : lvl) (Γ : Γ) vl (Rc : RC.t) (t : Λ) (τ : Τ) :
+Theorem weakening_ℜ_gen (k k' : lvl) (Γ : Γ) (Re Re1 : ℜ) (t : Λ) (τ : Τ) :
 
-        (* (1) *) k <= (RC.threshold Rc) ->  
-        (* (2) *) k <= k' -> 
-        (* (3) *) k' - k = (RC.threshold (RC.multi_add vl Rc)) - (RC.threshold Rc) ->
-        (* (5) *) Γ ⋅ Rc ⊢ t ∈ τ -> 
+        (* (1) *) k <= Re⁺ ->  (* (2) *) k <= k' -> (* (3) *) k' - k = Re1⁺ - Re⁺ ->
+         (* (4) *) (([⧐ k – (k' - k)] Re) ⊆ Re1)%rc -> (* (5) *) Γ ⋅ Re ⊢ t ∈ τ -> 
   (* ------------------------------------------------------------------------------------ *)
-       ([⧐ k – (k' - k)] Γ)%vc ⋅ 
-       (RC.multi_add vl Rc) ⊢ 
-      {Term.shift k (k' - k) t} ∈ [⧐ k – {k' - k}] τ.
+       ([⧐ k – (k' - k)] Γ)%vc ⋅ Re1 ⊢ {Term.shift k (k' - k) t} ∈ [⧐ k – {k' - k}] τ.
 Proof.
   intros Hle Hle' Heq Hsub wt; revert Re1 k k' Hle Hle' Hsub Heq.
   induction wt; intros Re1 n m Hle Hle' Hsub Heq; simpl; auto.
@@ -362,12 +257,12 @@ Proof.
   (* abstraction *)
   - constructor.
     -- rewrite <- VC.shift_add; now apply IHwt.
-    -- assert ((RC.threshold Rc) <= Re1⁺).
+    -- assert (Re⁺ <= Re1⁺).
        { 
          apply RC.Ext.new_key_Submap in Hsub. 
          now rewrite <- RC.shift_new_key_le in Hsub.
        }
-       apply (Typ.shift_preserves_wf_gen ((RC.threshold Re))); auto; lia. 
+       apply (Typ.shift_preserves_wf_gen (Re⁺)); auto; lia. 
   (* application *)
   - apply wt_app with (α := <[[⧐n – {m - n}] α]>); auto.
   (* fst *)
@@ -376,12 +271,12 @@ Proof.
   - simpl in *; apply wt_snd with (α := <[[⧐ n – {m - n}] α]>); auto.
   (* first *)
   - econstructor; eauto. 
-    assert ((RC.threshold Re) <= Re1⁺).
+    assert (Re⁺ <= Re1⁺).
     { 
       apply RC.Ext.new_key_Submap in Hsub. 
       now rewrite <- RC.shift_new_key_le in Hsub.
     }
-    apply Typ.shift_preserves_wf_gen with ((RC.threshold Re)); auto; lia.
+    apply Typ.shift_preserves_wf_gen with (Re⁺); auto; lia.
   (* comp *)
   - econstructor; eauto.
     -- rewrite <- Resources.shift_union.
@@ -393,7 +288,7 @@ Proof.
     apply RC.Submap_find with (m :=  ([⧐ n – m - n] Re)); auto.
     apply RC.shift_find_iff with (lb := n) (k := m - n) in H; auto.
   (* wormhole *)
-  - assert (Hle1 : (RC.threshold Re) <= Re1⁺). 
+  - assert (Hle1 : Re⁺ <= Re1⁺). 
     { 
       apply RC.Ext.new_key_Submap in Hsub. 
       now rewrite <- RC.shift_new_key_le in Hsub.
@@ -403,22 +298,22 @@ Proof.
        repeat rewrite Resources.shift_add_notin.
        + unfold Resource.shift. 
          rewrite <- Nat.leb_le in Hle; rewrite Hle.
-         replace (n <=? S ((RC.threshold Re))) with true.
+         replace (n <=? S (Re⁺)) with true.
          ++ rewrite Resources.shift_empty. 
             rewrite Heq; simpl.
-            now replace ((RC.threshold Re) + (Re1⁺ - (RC.threshold Re))) with (Re1⁺) by lia.
+            now replace (Re⁺ + (Re1⁺ - Re⁺)) with (Re1⁺) by lia.
         ++ symmetry; rewrite Nat.leb_le in *; lia.
       + intro HIn; inversion HIn.
       + rewrite Resources.St.add_notin_spec; split; auto. 
         intro HIn; inversion HIn.
-    -- apply Typ.shift_preserves_wf_gen with ((RC.threshold Re)); auto; lia.
-    -- apply Typ.shift_preserves_wf_gen with ((RC.threshold Re)); auto; lia.
+    -- apply Typ.shift_preserves_wf_gen with (Re⁺); auto; lia.
+    -- apply Typ.shift_preserves_wf_gen with (Re⁺); auto; lia.
     -- apply IHwt2; rewrite RC.new_key_wh in *; try lia. 
        + repeat rewrite RC.shift_add_notin.
          ++ unfold PairTyp.shift; simpl; unfold Resource.shift.
-           replace (n <=? S ((RC.threshold Re))) with true; replace (n <=? (RC.threshold Re)) with true;
+           replace (n <=? S (Re⁺)) with true; replace (n <=? Re⁺) with true;
            try (symmetry; rewrite Nat.leb_le; lia).
-           replace ((RC.threshold Re) + (m - n)) with (Re1⁺) by lia.
+           replace (Re⁺ + (m - n)) with (Re1⁺) by lia.
            replace (S (Re ⁺) + (m - n)) with (S (Re1⁺)) by lia.
            now repeat apply RC.Submap_add.
         ++ apply RC.Ext.new_key_notin; lia.
@@ -429,88 +324,54 @@ Qed.
 
 (** *** Weakening corollaries *)
 
-Corollary weakening_Γ_empty (Γ : Γ) (Re : RC.t) (t : Λ) (τ : Τ) :
+Corollary weakening_Γ_empty (Γ : Γ) (Re : ℜ) (t : Λ) (τ : Τ) :
 
        (∅)%vc ⋅ Re ⊢ t ∈ τ -> 
   (* -------------------------- *)
           Γ ⋅ Re ⊢ t ∈ τ.
 Proof. apply weakening_Γ; apply VContext.Submap_empty_bot. Qed.
 
-Corollary weakening_RC_1 (Γ : Γ) (Re Re1 : RC.t) (t : Λ) (τ : Τ) :
+Corollary weakening_ℜ_1 (Γ : Γ) (Re Re1 : ℜ) (t : Λ) (τ : Τ) :
 
-                ((RC.threshold Re) ⊩ Re)%rc -> (Re ⊆ Re1)%rc -> Γ ⋅ Re ⊢ t ∈ τ -> 
+                (Re⁺ ⊩ Re)%rc -> (Re ⊆ Re1)%rc -> Γ ⋅ Re ⊢ t ∈ τ -> 
 (* ---------------------------------------------------------------------------------- *)
-     ([⧐ (RC.threshold Re) – (Re1⁺ - (RC.threshold Re))] Γ)%vc ⋅ Re1 ⊢ 
-               {Term.shift ((RC.threshold Re)) (Re1⁺ - (RC.threshold Re)) t} ∈ ([⧐ {(RC.threshold Re)} – {Re1⁺ - (RC.threshold Re)}] τ)%ty.
+     ([⧐ Re⁺ – (Re1⁺ - Re⁺)] Γ)%vc ⋅ Re1 ⊢ 
+               {Term.shift (Re⁺) (Re1⁺ - Re⁺) t} ∈ ([⧐ {Re⁺} – {Re1⁺ - Re⁺}] τ)%ty.
 Proof. 
-  intros HvRe Hsub Hwt; apply weakening_RC.t_gen with (Re := Re); auto.
+  intros HvRe Hsub Hwt; apply weakening_ℜ_gen with (Re := Re); auto.
   - now apply RC.Ext.new_key_Submap.
   - rewrite RC.shift_wf_refl; auto.
 Qed.
 
-Corollary weakening_RC (Γ : Γ) (Re Re1 : RC.t) (t : Λ) (τ : Τ) :
+Corollary weakening_ℜ (Γ : Γ) (Re Re1 : ℜ) (t : Λ) (τ : Τ) :
 
-       ((RC.threshold Re) ⊩ Γ)%vc -> ((RC.threshold Re) ⊩ Re)%rc -> (Re ⊆ Re1)%rc -> Γ ⋅ Re ⊢ t ∈ τ -> 
+       (Re⁺ ⊩ Γ)%vc -> (Re⁺ ⊩ Re)%rc -> (Re ⊆ Re1)%rc -> Γ ⋅ Re ⊢ t ∈ τ -> 
   (* ----------------------------------------------------------------------- *)
-              Γ ⋅ Re1 ⊢ {Term.shift ((RC.threshold Re)) (Re1⁺ - (RC.threshold Re)) t} ∈ τ.
+              Γ ⋅ Re1 ⊢ {Term.shift (Re⁺) (Re1⁺ - Re⁺) t} ∈ τ.
 Proof.
   intros HvΓ HvRe Hsub Hwt.
-  apply (weakening_RC.t_1 _ _ Re1) in Hwt as Hwt'; auto.
+  apply (weakening_ℜ_1 _ _ Re1) in Hwt as Hwt'; auto.
   rewrite VC.shift_wf_refl in Hwt'; auto.
   apply well_typed_implies_Wf in Hwt as [_ Hvτ]; auto.
   now rewrite Typ.shift_wf_refl in Hwt'. 
 Qed.
 
-Corollary weakening_RC.t_2 (k k' : lvl) (Γ : Γ) (Re Re1 : RC.t) (t : Λ) (τ : Τ) :
+Corollary weakening_ℜ_2 (k k' : lvl) (Γ : Γ) (Re Re1 : ℜ) (t : Λ) (τ : Τ) :
 
-      ((RC.threshold Re) ⊩ Γ)%vc -> ((RC.threshold Re) ⊩ Re)%rc -> k = (RC.threshold Re) -> k' = Re1⁺ - (RC.threshold Re) ->
+      (Re⁺ ⊩ Γ)%vc -> (Re⁺ ⊩ Re)%rc -> k = Re⁺ -> k' = Re1⁺ - Re⁺ ->
                 (Re ⊆ Re1)%rc -> Γ ⋅ Re ⊢ t ∈ τ -> 
   (* ------------------------------------------------------------------ *) 
                 Γ ⋅ Re1 ⊢ {Term.shift k k' t} ∈ τ.
-Proof. intros; subst; now apply weakening_RC.t. Qed.
+Proof. intros; subst; now apply weakening_ℜ. Qed.
 
-Corollary weakening_RC.t_wh (Γ : Γ) (Re : RC.t) (t : Λ) (α β τ : Τ) :
+Corollary weakening_ℜ_wh (Γ : Γ) (Re : ℜ) (t : Λ) (α β τ : Τ) :
 
-                ((RC.threshold Re) ⊩ Γ)%vc -> ((RC.threshold Re) ⊩ Re)%rc -> Γ ⋅ Re ⊢ t ∈ τ -> 
+                (Re⁺ ⊩ Γ)%vc -> (Re⁺ ⊩ Re)%rc -> Γ ⋅ Re ⊢ t ∈ τ -> 
   (* ------------------------------------------------------------------------------- *)
-       Γ ⋅ (⌈S ((RC.threshold Re)) ⤆ (β, α)⌉ (⌈(RC.threshold Re) ⤆ (α, β)⌉ Re)) ⊢ {Term.shift ((RC.threshold Re)) 2 t} ∈ τ.
+       Γ ⋅ (⌈S (Re⁺) ⤆ (β, α)⌉ (⌈Re⁺ ⤆ (α, β)⌉ Re)) ⊢ {Term.shift (Re⁺) 2 t} ∈ τ.
 Proof.
   intros HvΓ HvRe Hwt.
-  apply (weakening_RC.t_2 _ _ _ Re); auto.
+  apply (weakening_ℜ_2 _ _ _ Re); auto.
   - rewrite RC.new_key_wh; lia.
   - apply RC.Submap_wh.
 Qed.
-
-
-(* Theorem weakening_RC.t_gen' (k k' : lvl) (Γ : Γ) (Re Re1 : RC.t) (t : Λ) (τ : Τ) :
-
-        (* (1) *) k <= (RC.threshold Re) ->  (* (2) *) k <= k' -> (* (3) *) k' - k = Re1⁺ - (RC.threshold Re) ->
-         (* (4) *) (([⧐ k – (k' - k)] Re) ⊆ Re1)%rc -> (* (5) *)
-          ([⧐ k – (k' - k)] Γ)%vc ⋅ Re1 ⊢ {Term.shift k (k' - k) t} ∈ [⧐ k – {k' - k}] τ -> 
-  (* ------------------------------------------------------------------------------------ *)
-        Γ ⋅ Re ⊢ t ∈ τ .
-Proof.
-  revert k k' Γ Re Re1 τ; induction t;
-  intros k k' Γ Re Re1 τ Hle Hle' Heq Hsub Hwt.
-  - simpl in *; inversion Hwt; subst.
-    destruct τ; inversion H1.
-    constructor.
-  - simpl in *; inversion Hwt; subst.
-    apply VC.shift_find_iff in H2.
-    constructor; auto.
-  - simpl in *; inversion Hwt; subst.
-    destruct τ; inversion H3; subst.
-    constructor.
-    -- eapply IHt; eauto.
-       rewrite VC.shift_add; auto.
-    -- admit.
-  - admit.
-  - admit.
-  - admit.
-  - admit.
-  - admit.
-  - admit.
-  - admit.
-  - simpl in *; inversion Hwt; subst.
-    destruct τ; inversion H2; subst; clear H2.
-      *)
