theories/Environment/GenEnv.v
@@ -1,3 +1,0 @@
-From Coq Require Import Classes.Morphisms.
-From Mecha Require Import Resource Typ Var.
-From DeBrLevel Require Import LevelInterface MapLevelInterface MapLevelD.
