theories/Environment/Saves.v
@@ -1,4 +1,0 @@
-From Coq Require Import Lia RelationClasses Classes.Morphisms.
-From Mecha Require Import Resource Term Typ RContext Save.
-From DeBrLevel Require Import LevelInterface.
-Import ResourceNotations TermNotations TypNotations RContextNotations.
